src/LogLayout.v
@@ -1,0 +1,191 @@
+Require Import CpdtTactics.
+Require Import FsTactics.
+Require Import DiskMod.
+Require Import Util.
+Require Import Smallstep.
+Require Import Closures.
+Require Import Tactics.
+Require Import LogPartsMod.
+Require Import FsLayout.
+Open Scope fscq.
+
+
+Definition LogHeader := 2.
+Definition LogEntries := 20.
+Definition SizeLogEntry := 2.
+
+
+Module LogPartSize <: DiskSize.
+Definition Size := LogHeader + LogEntries * SizeLogEntry.
+End LogPartSize.
+
+Module WholeDiskSize <: DiskSize.
+Definition Size := LogPartSize.Size + FsDiskSize.Size.
+End WholeDiskSize.
+
+
+Module LogPartDisk := Disk LogPartSize.
+Module LogPartsDisk := LogParts LogPartDisk FsDisk.
+Module WholeDisk := Disk WholeDiskSize.
+
+
+Ltac unfold_loglayout :=
+  unfold WholeDiskSize.Size in *;
+  unfold LogPartSize.Size in *;
+  unfold LogHeader in *;
+  unfold LogEntries in *;
+  unfold SizeLogEntry in *;
+  unfold_fslayout.
+
+Ltac omega'log :=
+  omega'unfold unfold_loglayout.
+
+Module LogPartsOnDisk <: Refines LogPartsDisk WholeDisk.
+
+Obligation Tactic := Tactics.program_simpl; omega'log.
+
+Program Definition l2w (n:LogPartDisk.addr) : WholeDisk.addr :=
+  n.
+
+Program Definition d2w (n:FsDisk.addr) : WholeDisk.addr :=
+  n + LogPartSize.Size.
+
+Ltac omega''log := unfold l2w in *; unfold d2w in *; auto; omega'log.
+
+Fixpoint CompileL (R T:Type) (p:LogPartDisk.Prog T)
+                             (rx:T->WholeDisk.Prog R) : WholeDisk.Prog R :=
+  match p with
+  | LogPartDisk.Read n rx' =>
+    a <- WholeDisk.Read (l2w n) ;
+    CompileL R T (rx' a) rx
+  | LogPartDisk.Write n b rx' =>
+    WholeDisk.Write (l2w n) b ;;
+    CompileL R T (rx' tt) rx
+  | LogPartDisk.Return r =>
+    rx r
+  end.
+
+Fixpoint CompileD (R T:Type) (p:FsDisk.Prog T)
+                             (rx:T->WholeDisk.Prog R) : WholeDisk.Prog R :=
+  match p with
+  | FsDisk.Read n rx' =>
+    a <- WholeDisk.Read (d2w n) ;
+    CompileD R T (rx' a) rx
+  | FsDisk.Write n b rx' =>
+    WholeDisk.Write (d2w n) b ;;
+    CompileD R T (rx' tt) rx
+  | FsDisk.Return r =>
+    rx r
+  end.
+
+Fixpoint Compile {R:Type} (p:LogPartsDisk.Prog R) : (WholeDisk.Prog R) :=
+  match p with
+  | LogPartsDisk.L T p rx => CompileL R T p (fun x => Compile (rx x))
+  | LogPartsDisk.D T p rx => CompileD R T p (fun x => Compile (rx x))
+  | LogPartsDisk.Return r => WholeDisk.Return r
+  end.
+
+Inductive statematch : LogPartsDisk.State -> WholeDisk.State -> Prop :=
+  | Match: forall ls ds d
+    (L: forall (a:LogPartDisk.addr), ls a = d (l2w a))
+    (D: forall (a:FsDisk.addr), ds a = d (d2w a)),
+    statematch (LogPartsDisk.PartState ls ds) d.
+Definition StateMatch := statematch.
+Hint Constructors statematch.
+
+Ltac resolve_disks :=
+  intros;
+  match goal with
+  | [ |- setidx ?eq _ ?a _ ?b = _ ] => destruct (eq a b)
+  | [ |- _ = setidx ?eq _ ?a _ ?b ] => idtac
+  end;
+  repeat resolve_setidx omega''log; auto.
+
+Theorem FSim:
+  forall R,
+  forward_simulation (LogPartsDisk.Step R) (WholeDisk.Step R).
+Proof.
+  intros; fsim_begin (@Compile R) statematch.
+
+  - (* L *)
+    generalize dependent s2. generalize dependent S.
+    generalize dependent ls. generalize dependent ds.
+    unfold Compile; fold (@Compile R).
+    induction p.
+
+    + intros; simpl;
+      edestruct H; inversion S; clear S;
+      match goal with
+      | [ H: star (?STEP R) _ _ |- _ ] =>
+        inversion H; match goal with
+        | [ Hstep: STEP _ _ _ |- _ ] => inversion Hstep
+        end
+      end; subst;
+      [ constructor; eauto
+      | instantiate (1:=s2); eauto
+      | instantiate (2:=ds); eauto
+      | exists x; split;
+        [ eapply star_step; [constructor|crush] | crush ] ].
+    + intros; simpl;
+      edestruct H; inversion S; clear S;
+      match goal with
+      | [ H: star (?STEP R) _ _ |- _ ] =>
+        inversion H; match goal with
+        | [ Hstep: STEP _ _ _ |- _ ] => inversion Hstep
+        end
+      end; subst;
+      [ constructor; eauto
+      | instantiate (1:=(setidx WholeDisk.eq_addr_dec s2 (l2w a) v)); resolve_disks
+      | instantiate (2:=ds); resolve_disks
+      | exists x; split;
+        [ eapply star_step; [constructor|crush] | crush ] ].
+    + intros; simpl;
+      inversion S; clear S; subst.
+      inversion STAR; [| match goal with
+                         | [ H: _ R (PS (_ v) _) _ |- _ ] => inversion H
+                         end ].
+      eexists; split; [ apply star_refl | constructor; crush ].
+
+  - (* D *)
+    generalize dependent s2. generalize dependent S.
+    generalize dependent ls. generalize dependent ds.
+    unfold Compile; fold (@Compile R).
+    induction p.
+
+    + intros; simpl;
+      edestruct H; inversion S; clear S;
+      match goal with
+      | [ H: star (?STEP R) _ _ |- _ ] =>
+        inversion H; match goal with
+        | [ Hstep: STEP _ _ _ |- _ ] => inversion Hstep
+        end
+      end; subst;
+      [ constructor; eauto
+      | instantiate (2:=ls);
+        instantiate (1:=s2); eauto
+      | eauto
+      | exists x; split;
+        [ eapply star_step; [constructor|crush] | crush ] ].
+    + intros; simpl;
+      edestruct H; inversion S; clear S;
+      match goal with
+      | [ H: star (?STEP R) _ _ |- _ ] =>
+        inversion H; match goal with
+        | [ Hstep: STEP _ _ _ |- _ ] => inversion Hstep
+        end
+      end; subst;
+      [ constructor; eauto
+      | instantiate (2:=ls);
+        instantiate (1:=(setidx WholeDisk.eq_addr_dec s2 (d2w a) v)); resolve_disks
+      | resolve_disks
+      | exists x; split;
+        [ eapply star_step; [constructor|crush] | crush ] ].
+    + intros; simpl;
+      inversion S; clear S; subst.
+      inversion STAR; [| match goal with
+                         | [ H: _ R (PS (_ v) _) _ |- _ ] => inversion H
+                         end ].
+      eexists; split; [ apply star_refl | constructor; crush ].
+Qed.
+
+End LogPartsOnDisk.
